speed

map_utils.dfy
@@ -11,6 +11,23 @@ module Map_Utils {
 		map x : U | (x in mapa.Keys + mapb.Keys) :: if x in mapa then mapa[x] else mapb[x]
 	}
 
+	// Requires disjoint domains and delivers predictable result.
+	function method {:opaque} disjoint_union3<U,T>(mapa: map<U,T>, mapb: map<U,T>, mapc: map<U,T>) : map<U,T>
+		requires mapa.Keys !! mapb.Keys !! mapc.Keys;
+		ensures disjoint_union3(mapa, mapb, mapc).Keys == mapa.Keys + mapb.Keys + mapc.Keys;
+		ensures mapa.Keys != {} || mapb.Keys != {} || mapc.Keys != {} ==> disjoint_union3(mapa, mapb, mapc).Keys != {};
+		ensures forall k :: k in mapa.Keys ==> mapa[k] == disjoint_union3(mapa, mapb, mapc)[k];
+		ensures forall k :: k in mapb.Keys ==> mapb[k] == disjoint_union3(mapa, mapb, mapc)[k];
+		ensures forall k :: k in mapc.Keys ==> mapc[k] == disjoint_union3(mapa, mapb, mapc)[k];
+		ensures disjoint_union3(mapa, mapb, mapc) == disjoint_union(mapa, disjoint_union(mapb, mapc))
+			                                        == disjoint_union(disjoint_union(mapa, mapb), mapc);
+	{
+		map x : U | (x in mapa.Keys + mapb.Keys + mapc.Keys) ::
+			if x in mapa then mapa[x]
+			else if x in mapb then mapb[x]
+			else mapc[x]
+	}
+
 	// Doesn't require disjoint domains, but guarantees to take A's
 	// definition.
 	function method {:opaque} union_preferA<U,T>(mapa: map<U,T>, mapb: map<U,T>) : map<U,T>
